graphs are now a sigma type.

graph_inst.v
@@ -2,7 +2,7 @@ Set Implicit Arguments.
 Require Import ZArith MSets.
 Require Import mgraphs_ind pair_UOT.
 
-Module Bleh : Graphs PositiveOrderedTypeBits.
+Module graph_inst : Graphs PositiveOrderedTypeBits.
   
   
   Module mset := MSetAVL.Make PositiveOrderedTypeBits.
@@ -20,9 +20,9 @@ Module Bleh : Graphs PositiveOrderedTypeBits.
   Definition node_set := mset.t.
   Definition node_setPair := msetPair.t.
 
-  Notation "[ ]" := mset.empty.
+  (* Notation "[ ]" := mset.empty. *)
 
-  Notation "[ elt0 , .. , eltn ]" := (mset.add elt0 .. (mset.add eltn (mset.empty )) .. ) (at level 60, right associativity).
+  (* Notation "[ elt0 , .. , eltn ]" := (mset.add elt0 .. (mset.add eltn (mset.empty )) .. ) (at level 60, right associativity). *)
 
   Inductive graph : Type :=
   | Empty : graph
@@ -31,266 +31,240 @@ Module Bleh : Graphs PositiveOrderedTypeBits.
       node_set -> (** its neighbors *)
       graph -> (** the rest of the graph *)
       graph.
-
-  Fixpoint vertices g : node_set :=
+(*vert to graph_vert*)
+    Fixpoint graph_vertices' g : node_set :=
     match g with
       | Empty => mset.empty
-      | Node x s g' => mset.add x (vertices g')
+      | Node x s g' => mset.add x (graph_vertices' g')
     end.
 
-  Fixpoint edges' g : node_setPair :=
-    match g with
-      | Empty => msetPair.empty
-      | Node x s g' =>  msetPair.union (mset.fold (fun x' s'=> msetPair.add (x,x') s') s msetPair.empty) (edges' g')
-    end.
+  
+  Inductive graph_ok : graph -> Prop :=
+  | EmptyOk : graph_ok Empty 
+  | NodeOk : forall (x : node) (adj : node_set) (g : graph),
+      graph_ok g ->
+      (forall (y : node), mset.In y adj -> mset.In y (graph_vertices' g)) ->
+      graph_ok (Node x adj g).
+  Definition valid_graph := {g : graph | graph_ok g}.
+  
+  Definition proj1 (vg : valid_graph) : graph :=
+    let (g, pf) := vg in g. 
 
-  Fixpoint edges g : node_setPair :=
-    match g with 
+  Definition project1 T: (graph -> T) -> (valid_graph -> T).
+    intros.
+    destruct X0.
+    apply X.
+    auto.
+    Defined.
+  
+  Definition graph_vertices (vg: valid_graph) := (project1 graph_vertices') vg.
+
+  Definition ok T: forall (vg : valid_graph) (g : graph) (f : graph -> T), f (proj1 vg) = (project1 f) vg.
+    intros.
+    destruct vg.
+    auto.
+    Defined.
+    
+Print ok.
+
+
+  (* Fixpoint edges' g : node_setPair := *)
+  (*   match g with *)
+  (*     | Empty => msetPair.empty *)
+  (*     | Node x s g' =>  msetPair.union (mset.fold (fun x' s'=> msetPair.add (x,x') s') s msetPair.empty) (edges' g') *)
+  (*   end. *)
+
+
+
+(*   Lemma node_ok_graph_ok : forall n adj g, graph_ok (Node n adj g) -> graph_ok g /\   (forall (y : node), mset.In y adj -> mset.In y (graph_vertices g)). *)
+(*   Proof. *)
+(*     intros. *)
+(*     split. *)
+(*     inversion H. *)
+(*     auto. *)
+(*     inversion H. *)
+(*     auto. *)
+(* Qed.     *)
+  Lemma emptyOk : graph_ok Empty.
+  Proof.
+    constructor.
+  Qed.
+
+  Definition t := valid_graph.
+  Definition empty : valid_graph.  
+  assert (graph_ok Empty).
+  constructor.
+  exists (Empty).
+  exact H.
+  Defined.
+
+    Fixpoint edges' ( g : graph) : node_setPair :=
+      match g with
       | Empty => msetPair.empty
       | Node x s g' => mset.fold (fun x' s' => msetPair.add (x,x') s')
-                        s (edges g')
+                        s (edges' g')
     end.
 
-  Definition t := graph.
-  Definition empty := Empty.
-  Definition add_vertex : t -> node -> t :=
+  Definition edges (vg : t) : node_setPair := edges' (proj1 vg).
+ 
+  Definition add_vertex' : graph -> node -> graph :=
     fun t x => Node x mset.empty t.
-  Definition add_edge: t -> node * node -> t :=
+
+
+
+
+  Theorem add_vertex_ok : forall v g, graph_ok g -> graph_ok (add_vertex' g v).
+  Proof.
+    intros.
+    induction g.
+    constructor.
+    auto.
+    intros y H1.
+    auto.
+    unfold add_vertex'.
+    constructor; auto.
+    intros y H1.
+    inversion H1.
+Qed.
+
+
+
+  
+  Definition add_vertex (vg : valid_graph) (v : node) : valid_graph. 
+  Proof.
+    exists (add_vertex' (proj1 vg) v).
+    apply add_vertex_ok.
+    destruct vg.
+    simpl.
+    exact g.
+    Defined.
+
+  Definition add_edge': graph -> node * node -> graph :=
     fun g (x : node*node)  =>
       let (x1, x2) := x in
-      if (mset.mem x1 (vertices g) && mset.mem x2 (vertices g))
+      if (mset.mem x1 (graph_vertices' g) && mset.mem x2 (graph_vertices' g))
       then Node x1 (mset.add x2 mset.empty) g
       else g.
-  Fixpoint remove_vertex (g : graph) (n : node) :=
-  match g with
-  |Empty => Empty
-  |Node n' adj g' => if Pos.eqb n' n then remove_vertex g' n
-      else  Node n' adj (remove_vertex g' n)
-  end.
 
-Fixpoint remove_edge (g : graph) (e : (node * node) ) :=
-  let x := (fst e) in
-  let y := (snd e) in
-  match g with
-  |Empty => Empty
-  |Node n adj g' => if Pos.eqb n x  then Node n (mset.remove y adj) (remove_edge g' e)
-                   else Node n adj (remove_edge g' e)
-  end.
+  Theorem add_edge_ok : forall e g, graph_ok g -> graph_ok (add_edge' g e).
+  Proof.
+    intros e g H.
+    destruct e.
+    induction g.
+    auto.
+    simpl.
+    destruct (mset.mem n (mset.add n1 (graph_vertices' g)) &&
+                        mset.mem n0 (mset.add n1 (graph_vertices' g))) eqn:H1.
+    apply andb_true_iff in H1.
+    destruct H1.
+    constructor.
+    auto.
+    intros y H2.
+    apply mset_prop.singleton_equal_add in H2.
+    apply mset_prop.Dec.F.singleton_1 in H2.
+    simpl.
+    subst.
+    apply mset.mem_spec.
+    auto.
+    auto.
+  Qed.
 
-
-Fixpoint neighborhood (g : graph) (x : node) : node_set:=
-  match g with
-  | Empty => mset.empty
-  | Node y adj g' =>
-    if Pos.eqb x y then  mset.union adj (neighborhood g' x)
-    else if mset.mem x adj then mset.add y (neighborhood g' x)
-         else neighborhood g' x
-  end.
+  Definition add_edge : valid_graph ->  node * node -> valid_graph.
+    intros.
+    exists (add_edge' (proj1 X) H).
+    apply add_edge_ok.
+    destruct X.
+    simpl.
+    exact g.
+    Defined.
   
+  
+
+  
+  
+  Fixpoint remove_vertex' (g : graph) (n : node) :=
+  match g with
+  |Empty => Empty
+  |Node n' adj g' => if Pos.eqb n' n then remove_vertex' g' n
+      else  Node n' adj (remove_vertex' g' n)
+  end.
+
+    Lemma remove_vertex_ok : forall g v, graph_ok g -> graph_ok (remove_vertex' g v).
+    Proof.
+      induction g.
+      constructor.
+      simpl.
+      intros.
+      destruct ((n =? v)%positive) eqn:H1.
+      apply IHg.
+      inversion H.
+      auto.
+      constructor.
+      inversion H.
+      auto.
+      intros.
+      inversion H.
+      subst.
+      apply (IHg v) in H4.
+    Admitted.
     
-  Definition is_vertex : t -> node -> bool :=
-    fun g x => mset.mem x (vertices g).
-  Definition is_edge : t -> node * node -> bool :=
-    fun g x => msetPair.mem x (edges g).
-  Lemma empty_vertices : vertices empty = mset.empty.
+
+  Definition remove_vertex (vg : t) (v : node) : t.  
+    exists (remove_vertex' (proj1 vg) v).
+    apply remove_vertex_ok.
+    destruct vg.
+    exact g.
+    Defined.
+
+  Fixpoint remove_edge' (g : graph) (e : (node * node) ) :=
+    let x := (fst e) in
+    let y := (snd e) in
+    match g with
+    |Empty => Empty
+    |Node n adj g' => if Pos.eqb n x  then Node n (mset.remove y adj) (remove_edge' g' e)
+                      else Node n adj (remove_edge' g' e)
+    end.
+
+  Lemma remove_edge_ok : forall (g : graph) ( e : (node * node)),
+      graph_ok g -> graph_ok (remove_edge' g e).
+  Proof.
+    Admitted.
+
+  Definition remove_edge (vg : t) (e : node * node ) : t.
+    exists (remove_edge' (proj1 vg) e).
+    apply remove_edge_ok.
+    destruct vg.
+    exact g.
+    Defined.
+  
+  Fixpoint neighborhood' (g : graph) (x : node) : node_set:=
+    match g with
+    | Empty => mset.empty
+    | Node y adj g' =>
+      if Pos.eqb x y then  mset.union adj (neighborhood' g' x)
+      else if mset.mem x adj then mset.add y (neighborhood' g' x)
+           else neighborhood' g' x
+    end.
+  Definition neighborhood := (project1 neighborhood').
+    
+  Definition is_vertex' : graph -> node -> bool :=
+    fun g x => mset.mem x (graph_vertices' g).
+  Definition is_vertex := (project1 is_vertex').
+  Definition is_edge' : graph -> node * node -> bool :=
+    fun g x => msetPair.mem x (edges' g).
+
+  Definition is_edge := (project1 is_edge').
+
+
+  Lemma empty_vertices : graph_vertices empty = mset.empty.
   Proof. reflexivity. Qed.
   Lemma empty_edges : edges empty = msetPair.empty.
   Proof. reflexivity. Qed.
 
-  Lemma node_edges_weaken : forall (g : t) (n x y : node) n0  (e :=(x, y) : node * node),
-      msetPair.In (x,y) (edges (Node n n0 g)) ->
-      x = n /\ mset.In y n0 \/ msetPair.In e (edges g).
-    Proof.
-      intros. simpl in H.
-    Admitted.
-
-  Lemma node_pres_verts : forall (n : node) (e : node_set) (g : t),
-      mset.Equal (vertices (Node n e g)) (mset.union (mset.add n mset.empty) (vertices g)).
-  Proof.
-    intros.
-    induction g.
-    simpl.
-    intros.
-    rewrite mset_prop.empty_union_2.
-    reflexivity. auto.
-    simpl.
-    intros.
-    rewrite mset_prop.add_union_singleton.
-    apply  mset_prop.union_equal_1.
-    apply mset_prop.singleton_equal_add.
-  Qed.
-
   Definition pairset_of_nodes (n : node) (e : node_set) :=
     mset.fold (fun (x : node) l => msetPair.add (n, x) l) e msetPair.empty.
 
-  Lemma node_pres_edges  : forall (n : node) (e : node_set)  (g : graph),
-      msetPair.Equal (edges (Node n e g))
-  (msetPair.union (pairset_of_nodes n e) (edges g)).
-  Proof.
-    intros.
-    simpl.
-    generalize (edges g).
-    intro n0.
-    set (P := fun e => ( msetPair.Equal
-     (mset.fold
-        (fun (x' : mset.elt) (s' : msetPair.t) =>
-         msetPair.add (n, x') s') e n0)
-     (msetPair.union (pairset_of_nodes n e) n0))).
-    change (P e).
-    apply mset_prop.set_induction.
-    intros.
-    unfold P.
-
-    rewrite mset_prop.fold_1b.
-    unfold pairset_of_nodes.
-    rewrite mset_prop.fold_1b.
-    rewrite msetPair_prop.empty_union_1.
-    reflexivity;
-    auto.
-    auto.
-    auto.
-    auto.
-    intros.
-    unfold P.
-    unfold pairset_of_nodes.
-    apply mset_prop.Add_Equal in H1.
-    rewrite mset_prop.fold_2.
-    Admitted.
-
-
-   Open Scope positive_scope.
-   Example ex1 : graph :=
-  Node 1 ([2,  3])
-       (Node 2 ([3])
-             (Node 3 [] Empty)).
-   
-   Compute (msetPair.elements (edges ex1)).
-   Compute (msetPair.elements (edges' ex1)).
-
-  Lemma add_vertices :
-    forall (x : node) (g : t), mset.In x (vertices (add_vertex g x)).
-  Proof.
-    intros.
-    induction g; simpl; apply mset.add_spec;
-    left; reflexivity.
-  Qed.
-
-  Lemma add_edges :
-    forall (e : node * node) (g : t),
-      mset.In (fst e) (vertices g) ->
-      mset.In (snd e) (vertices g) ->
-      msetPair.In e (edges (add_edge g e)).
-  Proof.
-    intros. destruct e.
-    induction g; simpl.
-    inversion H.
-    simpl in H, H0.
-    apply mset.add_spec in H.
-    apply mset.add_spec in H0.    
-    destruct H, H0.
-    rewrite H, H0.
-    {
-      assert ( mset.mem n1 (mset.add n1 (vertices g)) = true).
-      rewrite mset.mem_spec.
-      apply mset_prop.Dec.F.add_iff.
-      auto.
-      rewrite H1.
-
-      simpl ( _ && _).
-      cbv iota.
-      generalize (Node n1 n2 g).
-      intros.
-      
-      simpl.
-      apply msetPair.add_spec.
-      auto.
-    }
-    {
-       assert ( mset.mem n (mset.add n1 (vertices g)) = true).
-      rewrite mset.mem_spec.
-      apply mset_prop.Dec.F.add_iff.
-      auto.
-      rewrite H1.
-      assert (mset.mem n0 (mset.add n1 (vertices g)) = true).
-      rewrite mset.mem_spec.
-      apply mset_prop.Dec.F.add_iff.
-      auto.
-      rewrite H2.
-      simpl (_ && _); cbv iota.
-      generalize (Node n1 n2 g).
-      intro g0.
-      simpl.
-      apply msetPair.add_spec.
-      auto.
-    }
-    {
-      assert ( mset.mem n (mset.add n1 (vertices g)) = true).
-      rewrite mset.mem_spec.
-      apply mset_prop.Dec.F.add_iff.
-      auto.
-      rewrite H1.
-      assert (mset.mem n0 (mset.add n1 (vertices g)) = true).
-      rewrite mset.mem_spec.
-      apply mset_prop.Dec.F.add_iff.
-      auto.
-      rewrite H2.
-      simpl ( _ && _); cbv iota.
-      generalize (Node n1 n2 g).
-      intro g0.
-      simpl.
-      apply msetPair.add_spec.
-      auto.
-    }
-    {
-      
-      assert ( mset.mem n (mset.add n1 (vertices g)) = true).
-      rewrite mset.mem_spec.
-      apply mset_prop.Dec.F.add_iff.
-      auto.
-      rewrite H1.
-      assert (mset.mem n0 (mset.add n1 (vertices g)) = true).
-      rewrite mset.mem_spec.
-      apply mset_prop.Dec.F.add_iff.
-      auto.
-      rewrite H2.
-      simpl ( _ && _); cbv iota.
-       generalize (Node n1 n2 g).
-      intro g0.
-      simpl.
-      apply msetPair.add_spec.
-      auto.
-    }
-  Qed.
-
-    Lemma add_vertices_other :
-      forall (x y : node) (g : t),
-        x <> y -> mset.In y (vertices g) <-> mset.In y (vertices (add_vertex g x)).
-    Proof.
-      split; intros; induction g.
-      inversion H0.
-      {
-       unfold add_vertex.
-       simpl. apply mset.add_spec.
-       auto.
-      }
-      {
-       simpl.
-       inversion H0.
-       symmetry in H2;
-       contradiction.
-       auto. auto.
-      }
-       simpl. apply mset.add_spec.
-       unfold add_vertex in H0.
-       simpl in H0. apply mset.add_spec in H0.
-       destruct H0.
-       symmetry in H0.
-       contradiction.
-       apply mset.add_spec in H0.
-       auto.
-    Qed.
-
-    Lemma folds_equal : forall n n0 s ,
+  Lemma folds_equal : forall n n0 s ,
       msetPair.Equal
         ((mset.fold
           (fun (x' : mset.elt) (s' : msetPair.t) =>
@@ -303,6 +277,7 @@ Fixpoint neighborhood (g : graph) (x : node) : node_set:=
       {
         intros. rewrite H0.
         apply mset_prop.fold_equal with (s := s0) (s' := s').
+        
         admit.
         admit.
         admit.
@@ -319,59 +294,194 @@ Fixpoint neighborhood (g : graph) (x : node) : node_set:=
         rewrite msetPair.union_spec.
 Admitted.
 
+
+
+
+    (*   Open Scope positive_scope.*)
+  (*  Example ex1 : graph := *)
+  (* Node 1 ([2,  3]) *)
+  (*      (Node 2 ([3]) *)
+  (*            (Node 3 [] Empty)). *)
+   
+  (*  Compute (msetPair.elements (edges ex1)). *)
+  (*  Compute (msetPair.elements (edges' ex1)). *)
+
+  Lemma add_vertices :
+    forall (x : node) (g : t), mset.In x (graph_vertices (add_vertex g x)).
+  Proof.
+    intros.
+    induction g; simpl; apply mset.add_spec;
+    left; reflexivity.
+  Qed.
+
+  Lemma add_edges_aux :
+    forall n n0 n1 g,  n = n1 /\ mset.In n0 (graph_vertices' g) \/ n1 = n0 /\ mset.In n (graph_vertices' g) ->
+       mset.mem n (mset.add n1 (graph_vertices' g)) &&                              mset.mem n0 (mset.add n1 (graph_vertices' g)) = true.
+    Proof.
+      intros.
+      subst.
+      apply andb_true_iff.
+      destruct H;
+      destruct H;
+      split;
+      rewrite mset.mem_spec;
+      rewrite mset.add_spec;
+      auto.
+      Qed.
+
+
+  Lemma add_edges :
+    forall (e : node * node) (g : t),
+      mset.In (fst e) (graph_vertices g) ->
+      mset.In (snd e) (graph_vertices g) ->
+      msetPair.In e (edges (add_edge g e)).
+  Proof.
+    intros. destruct e.
+    destruct g as [g  pf].
+    unfold edges; unfold add_edge;
+    induction g; simpl.
+    simpl in H, H0.
+    inversion H.
+    simpl in H, H0.
+    apply mset.add_spec in H.
+    apply mset.add_spec in H0.    
+    destruct H, H0.
+    {
+      assert ( mset.mem n (mset.add n1 (graph_vertices' g)) = true).
+      rewrite mset.mem_spec.
+      apply mset_prop.Dec.F.add_iff.
+      auto. subst.
+      rewrite H1.
+      simpl ( _ && _).
+      cbv iota.
+      apply msetPair.add_spec.
+      auto.
+    }    
+   
+      rewrite add_edges_aux; auto.
+      generalize (Node n1 n2 g);
+      intro g0;
+      simpl;
+      apply msetPair.add_spec;
+      auto.
+    {
+      rewrite add_edges_aux; auto.
+      generalize (Node n1 n2 g).
+      intro g0;
+      simpl;
+      apply msetPair.add_spec;
+      auto.
+    }
+    {
+      assert ( mset.mem n (mset.add n1 (graph_vertices' g)) = true).
+      rewrite mset.mem_spec.
+      apply mset_prop.Dec.F.add_iff.
+      auto.
+      rewrite H1.
+      assert (mset.mem n0 (mset.add n1 (graph_vertices' g)) = true).
+      rewrite mset.mem_spec.
+      apply mset_prop.Dec.F.add_iff.
+      auto.
+      rewrite H2.
+      simpl ( _ && _); cbv iota.
+      generalize (Node n1 n2 g).
+      intro g0.
+      simpl.
+      apply msetPair.add_spec.
+      auto.
+    }
+  Qed.
+
+    Lemma add_vertices_other :
+      forall (x y : node) (g : t),
+        x <> y -> mset.In y (graph_vertices g) <-> mset.In y (graph_vertices (add_vertex g x)).
+    Proof.
+      split; intros; induction g.
+      inversion H0.
+      {
+       unfold add_vertex.
+       simpl. apply mset.add_spec.
+       auto.
+      }
+      {
+       simpl in H0.
+       inversion H0.
+       subst.
+       simpl.
+       apply mset.add_spec.
+       auto.
+       simpl.
+       apply mset.add_spec.
+       auto.
+       simpl.
+       apply mset.add_spec.
+       auto.
+      }
+       simpl. apply mset.add_spec.
+       unfold add_vertex in H0.
+       simpl in H0. auto.
+       simpl.
+       simpl in H0.
+       apply mset.add_spec in H0.
+       destruct H0.
+       symmetry in H0.
+       contradiction.
+       auto.
+    Qed.
+
     Lemma add_edges_other :
       forall (e1 e2 : node * node) (g : t),
         e1 <> e2 -> msetPair.In e2 (edges g) <-> msetPair.In e2 (edges (add_edge g e1)).
     Proof.
-      intros; split; induction g; auto.
+      intros; split.  destruct g as [g pf]. induction g; unfold edges in *; unfold add_edge in *; simpl.
       {
-       
-       inversion 1.
+        inversion 1.
       }
       {
         intros. unfold add_edge. 
         simpl.  destruct e1.
-        case_eq (mset.mem n1 (mset.add n (vertices g)));
-          case_eq ( mset.mem n2 (mset.add n (vertices g))).
-       
-        intros H1 H2; simpl (_ && _); cbv iota.
-          apply msetPair.add_spec;
-          auto.
-          auto.
-          auto. auto.
+        case_eq (mset.mem n1 (mset.add n (graph_vertices' g)));
+          case_eq ( mset.mem n2 (mset.add n (graph_vertices' g)));
+       simpl;
+        intros;
+        rewrite H1, H2;
+        simpl (_ && _); cbv iota;
+        simpl; auto;
+        apply msetPair.add_spec; auto.
       }
       {
+        simpl.
+        unfold edges, add_edge.
+        simpl.
         intros.
-        destruct e1.
-        auto.
-      }
-      {
-        intros.
+        unfold add_edge' in H0.
         apply msetPair_prop.Dec.F.add_3 with (x := e1).
         auto. rewrite msetPair.add_spec.
         right.
-        rewrite node_pres_edges.
-        apply msetPair.union_spec.
-        unfold add_edge in H0.
         destruct e1, e2.
-        destruct ( mset.mem n1 (vertices (Node n n0 g)) &&
-                            mset.mem n2 (vertices (Node n n0 g))) in H0.
+        destruct g as [g pf].
+        simpl in *.
+        destruct (mset.mem n (graph_vertices' g) && mset.mem n0 (graph_vertices' g)) eqn:H1.
+        apply folds_equal in H0.
+        apply msetPair.union_spec in H0.
+        fold edges' in H0.
+        destruct H0.
+        unfold pairset_of_nodes in H0.
+        rewrite mset.fold_spec in H0.
         simpl in H0.
-        apply  msetPair.add_spec in H0.
+        Focus 2.
+        auto.
+        Focus 2.
+        auto.
+        apply msetPair.add_spec in H0.
         destruct H0.
         symmetry in H0.
-        unfold not in H.
         apply H in H0.
         destruct H0.
-        apply msetPair.union_spec.
-        unfold pairset_of_nodes.
-        apply  folds_equal.
-        auto. (*Above lemma needs to be proven*)
-        apply node_pres_edges in H0.
-        apply msetPair.union_spec.
-        auto.
-      }
+        inversion H0.
+        }
     Qed.
+
 
     Lemma add_vertices_pres_edges :
       forall (x : node) (g : t), msetPair.Equal (edges (add_vertex g x)) (edges g).
@@ -382,40 +492,40 @@ Admitted.
     
     Lemma add_edges_pres_vertices :
       forall (x : node * node) (g : t),
-        mset.Equal (vertices (add_edge g x)) (vertices g).
+        mset.Equal (graph_vertices (add_edge g x)) (graph_vertices g).
     Proof.
       intros.
+      destruct g as [g pf].
       unfold add_edge. destruct x.
-      case_eq (mset.mem n (vertices g));
-      case_eq ( mset.mem n0 (vertices g)).
+      simpl.
+      case_eq (mset.mem n (graph_vertices' g));
+      case_eq ( mset.mem n0 (graph_vertices' g)); try (reflexivity).
       {
-        intros H1 H2; simpl. 
+        intros H1 H2; simpl.
         apply mset.mem_spec in H2.
         apply mset_prop.add_equal.
         auto.
       }
-      {
-        reflexivity.
-      }
-      {
-        reflexivity.
-      }
-      reflexivity.
     Qed.
          
     Lemma remove_vertices :
-      forall (x : node) (g : t), ~ mset.In x (vertices (remove_vertex g x)).
+      forall (x : node) (g : t), ~ mset.In x (graph_vertices (remove_vertex g x)).
     Proof.
       intros.
+      unfold graph_vertices, remove_vertex.
+      destruct g as [ g pf].
       induction g.
       simpl.
       inversion 1.
       unfold not in *.
       intros.
       simpl in H.
-      case_eq (n =? x).
+      case_eq ((n =? x)%positive).
       intros.
       rewrite H0 in H.
+      simpl in IHg.
+      apply Peqb_true_eq in H0.
+      inversion pf. subst.
       auto.
       intros.
       rewrite H0 in H.
@@ -425,18 +535,33 @@ Admitted.
       apply Pos.eqb_neq in H0.
       unfold not in H0.
       auto.
+      simpl in *.
+      inversion pf. subst.
       auto.
-Qed.
+    Qed.
     
     Lemma remove_edges :
       forall (e : node * node) (g : t), ~ msetPair.In e (edges (remove_edge g e)).
     Proof.
       intros.
-      unfold not. intros. induction g.
+      destruct e.
+      unfold not, remove_edge. intros. destruct g as [g pf].
+      induction g.
       inversion H.
-      simpl in H.
-      apply IHg.
-   Admitted.
+      simpl in *.
+      inversion pf. subst.
+      apply IHg with (pf := H2).
+      case_eq ((n1 =? n)%positive).
+      intros.
+      apply Peqb_true_eq in H0.
+      subst.
+      assert ((n =? n)%positive = true).
+      apply Pos.eqb_refl.
+      Focus 2.
+      intros.
+      apply Pos.eqb_neq in H0.
+      apply Pos.eqb_neq in H0.
+    Admitted.
 
 
     Lemma remove_vertices_edges_l :
@@ -460,16 +585,18 @@ Qed.
       intros.
       induction g.
       inversion H.
-      apply IHg; auto.
       simpl in H.
       
     Admitted.
 
     Lemma remove_vertices_other :
         forall (x y : node) (g : t),
-          x <> y ->  mset.In y (vertices g) <-> mset.In y (vertices (remove_vertex g x)).
+          x <> y ->  mset.In y (graph_vertices g) <-> mset.In y (graph_vertices (remove_vertex g x)).
     Proof.
       intros.
+      destruct g as [g pf].
+      unfold graph_vertices, remove_vertex.
+      simpl.
       split. intros.
       induction g.
       auto. simpl.
@@ -477,7 +604,7 @@ Qed.
       rewrite mset.add_spec in H0.
       destruct H0.
       {
-        destruct (n =? x) eqn:H1.
+        destruct ((n =? x)%positive) eqn:H1.
         apply Peqb_true_eq in H1.
         rewrite H1 in H0.
         unfold not in H.
@@ -490,10 +617,12 @@ Qed.
       }
       {
         apply IHg in H0.
-        destruct (n =? x) eqn:H1.
+        destruct ((n =? x)%positive) eqn:H1.
         auto.
         simpl.
         apply mset.add_spec.
+        auto.
+        inversion pf.
         auto.
       }
       induction g.
@@ -501,25 +630,37 @@ Qed.
       inversion H0.
       intro H0.
       unfold remove_vertex in H0.
-      case_eq (n =? x); intros H1;
-      rewrite H1 in H0; fold remove_vertex in H0.
-      admit.
       simpl in *.
-    Admitted.
-    
-    Lemma in_edge_node_or_graph :
-      forall (g : t) n n0(e : node * node) ,
-        msetPair.In e (edges (Node n n0 g)) ->
-          (msetPair.In e (pairset_of_nodes n n0) \/ msetPair.In e (edges g)).
-    Proof.
-      intros.
-      generalize dependent g.
-      generalize dependent n.
-      generalize dependent n0.
-      induction g.
+      case_eq ((n =? x)%positive); intros H1.
+      rewrite H1 in H0.
+      apply mset.add_spec.
+      right.
+      inversion pf. subst.
+      apply IHg; auto.
+      rewrite H1 in H0.
+      simpl in *.
+      rewrite mset.add_spec.
+      rewrite mset.add_spec in H0.
+      destruct H0.
       auto.
-      intros.
-      Admitted.
+      right.
+      inversion pf.
+      apply IHg; auto.
+    Qed.
+    
+    (* Lemma in_edge_node_or_graph : *)
+    (*   forall (g : t) n n0(e : node * node) , *)
+    (*     msetPair.In e (edges (Node n n0 g)) -> *)
+    (*       (msetPair.In e (pairset_of_nodes n n0) \/ msetPair.In e (edges g)). *)
+    (* Proof. *)
+    (*   intros. *)
+    (*   generalize dependent g. *)
+    (*   generalize dependent n. *)
+    (*   generalize dependent n0. *)
+    (*   induction g. *)
+    (*   auto. *)
+    (*   intros. *)
+    (*   Admitted. *)
       
 
 Lemma remove_edges_other :
@@ -527,35 +668,25 @@ Lemma remove_edges_other :
         e1 <> e2 -> msetPair.In e2 (edges g) <-> msetPair.In e2 (edges (remove_edge g e1)).
     Proof.
       intros. destruct e1,e2.
+      destruct g as [g pf].
       induction g.
       {
+        split.
+        auto.
         auto.
       }
       {
+        split.
         intro H1.
         simpl.
-        rewrite node_pres_edges in H1.
-        rewrite msetPair.union_spec in H1.
         destruct H1.
-        destruct (n3 =? n) eqn:H2.
-        {
-          rewrite node_pres_edges.
-          apply msetPair.union_spec.
-          left.
-          unfold pairset_of_nodes.
-          rewrite folds_equal.
-          rewrite msetPair.union_spec.
-          left.
-        admit.
-      }
-      {
-        auto.
       Admitted.
 
 
       Lemma is_vertex_vertices :
-        forall (x : node) (g : t), mset.In x (vertices g) <-> is_vertex g x = true.
+        forall (x : node) (g : t), mset.In x (graph_vertices g) <-> is_vertex g x = true.
       Proof.
+        destruct g as [g pf].
         intros;
         split; apply mset.mem_spec.
       Qed.
@@ -563,7 +694,7 @@ Lemma remove_edges_other :
       Lemma is_edge_edges :
         forall (e : node * node ) (g : t), msetPair.In e (edges g) <-> is_edge g e = true.
       Proof.
-        intros.
+        intros. destruct g as [g pf].
         split; apply msetPair.mem_spec.
       Qed.
       
@@ -572,23 +703,22 @@ Lemma remove_edges_other :
         forall (x : node) (y : node) (g : t),
           mset.In y (neighborhood g x) <-> msetPair.In (x, y) (edges g).
       Proof.
-        intros; split. intros. 
-        induction g.
-        inversion H.
-        rewrite node_pres_edges.
-        rewrite msetPair.union_spec .
-
-        admit.
         intros.
-        induction g.
-        inversion H.
-        simpl.
       Admitted.        
 
+
+      Lemma node_edges_weaken : forall (g : graph) (n x y : node) n0  (e :=(x, y) : node * node),
+      msetPair.In (x,y) (edges' (Node n n0 g)) ->
+      x = n /\ mset.In y n0 \/ msetPair.In e (edges' g).
+    Proof.
+      intros. simpl in H.
+    Admitted.
+      
       Lemma edges_proper_l :
-        forall (e : node * node) (g : t), msetPair.In e (edges g) -> mset.In (fst e) (vertices g).
+        forall (e : node * node) (g : t), msetPair.In e (edges g) -> mset.In (fst e) (graph_vertices g).
       Proof.
         intros.
+        destruct g as [g pf].
         induction g.
         inversion H.
         destruct e.
@@ -598,27 +728,31 @@ Lemma remove_edges_other :
         apply mset.add_spec. 
         destruct H.
         auto.
-        apply IHg in H.
+        inversion pf.
+        apply IHg with (pf := H2) in H.
         simpl.
         apply mset.add_spec.
         auto.
 Qed.
       Lemma edges_proper_r :
-        forall (e : node * node ) (g : t), msetPair.In e (edges g) -> mset.In (snd e) (vertices g).
+        forall (e : node * node ) (g : t), msetPair.In e (edges g) -> mset.In (snd e) (graph_vertices g).
       Proof.
         intros.
+        destruct g as [g pf].
         induction g.
+        intros.
         inversion H.
         simpl.
         destruct e.
         apply  node_edges_weaken in H.
         destruct H.
         simpl; apply mset.add_spec.
+        destruct H.
+        right.
         Admitted.
 
-
-End Bleh.
+End graph_inst.
 Print Graphs.
 
-Module graph_prop := graph_properties  PositiveOrderedTypeBits Bleh.
+Module graph_prop := graph_properties  PositiveOrderedTypeBits graph_inst.
 Print graph_prop.
